matching-logic/src/ProofSystem.v
@@ -326,6 +326,66 @@ Proof. intros H. rewrite <- e in H. exact H. Defined.
     | Singleton_ctx _ _ _ _ _ _ => false
     end.
 
+    Fixpoint propositional_only Γ ϕ (pf : Γ ⊢ ϕ) :=
+      match pf with
+      | hypothesis _ _ _ _ => true
+      | P1 _ _ _ _ _ => true
+      | P2 _ _ _ _ _ _ _ => true
+      | P3 _ _ _ => true
+      | Modus_ponens _ _ _ m0 m1
+        => propositional_only _ _ m0 && propositional_only _ _ m1
+      | Ex_quan _ _ _ _ => false
+      | Ex_gen _ _ _ _ _ _ pf' _ => false
+      | Prop_bott_left _ _ _ => false
+      | Prop_bott_right _ _ _ => false
+      | Prop_disj_left _ _ _ _ _ _ _ => false
+      | Prop_disj_right _ _ _ _ _ _ _ => false
+      | Prop_ex_left _ _ _ _ _ => false
+      | Prop_ex_right _ _ _ _ _ => false
+      | Framing_left _ _ _ _ _ m0 => false
+      | Framing_right _ _ _ _ _ m0 => false
+      | Svar_subst _ _ _ X _ _ m0 => false
+      | Pre_fixp _ _ _ => false
+      | Knaster_tarski _ _ phi psi m0 => false
+      | Existence _ => false
+      | Singleton_ctx _ _ _ _ _ _ => false
+      end.
+  
+  Lemma propositional_implies_noKT Γ ϕ (pf : Γ ⊢ ϕ) :
+    propositional_only Γ ϕ pf = true -> uses_kt Γ ϕ pf = false.
+  Proof.
+    induction pf; simpl; intros H; try reflexivity; try congruence.
+    { destruct_and!. rewrite IHpf1;[assumption|]. rewrite IHpf2;[assumption|]. reflexivity. }
+  Qed.
+
+  Lemma propositional_implies_no_uses_svar Γ ϕ (pf : ML_proof_system Γ ϕ) (SvS : SVarSet) :
+    propositional_only Γ ϕ pf = true -> uses_svar_subst SvS Γ ϕ pf = false.
+  Proof.
+    induction pf; simpl; intros H; try reflexivity; try congruence.
+    { destruct_and!. rewrite IHpf1;[assumption|]. rewrite IHpf2;[assumption|]. reflexivity. }
+  Qed.
+
+  Lemma propositional_implies_no_uses_ex_gen Γ ϕ (pf : ML_proof_system Γ ϕ) (EvS : EVarSet) :
+    propositional_only Γ ϕ pf = true -> uses_ex_gen EvS Γ ϕ pf = false.
+  Proof.
+    induction pf; simpl; intros H; try reflexivity; try congruence.
+    { destruct_and!. rewrite IHpf1;[assumption|]. rewrite IHpf2;[assumption|]. reflexivity. }
+  Qed.
+  
+  Lemma propositional_implies_no_uses_ex_gen_2 Γ ϕ (pf : ML_proof_system Γ ϕ) :
+    propositional_only Γ ϕ pf = true -> uses_of_ex_gen Γ ϕ pf = ∅.
+  Proof.
+    induction pf; simpl; intros H; try reflexivity; try congruence.
+    { destruct_and!. rewrite IHpf1;[assumption|]. rewrite IHpf2;[assumption|]. set_solver. }
+  Qed.
+
+  Lemma propositional_implies_no_uses_svar_2 Γ ϕ (pf : ML_proof_system Γ ϕ)  :
+    propositional_only Γ ϕ pf = true -> uses_of_svar_subst Γ ϕ pf = ∅.
+  Proof.
+    induction pf; simpl; intros H; try reflexivity; try congruence.
+    { destruct_and!. rewrite IHpf1;[assumption|]. rewrite IHpf2;[assumption|]. set_solver. }
+  Qed.
+
   Definition proofbpred := forall (Γ : Theory) (ϕ : Pattern),  Γ ⊢ ϕ -> bool.
 
   Definition indifferent_to_cast (P : proofbpred)
@@ -367,6 +427,18 @@ Proof. intros H. rewrite <- e in H. exact H. Defined.
      match type of e with
      | ?x = ?x => replace e with (@erefl _ x) by (apply UIP_dec; intros x' y'; apply Pattern_eqdec)
      end; simpl; try reflexivity.
+  Qed.
+
+  Lemma indifferent_to_cast_propositional_only :
+    indifferent_to_cast propositional_only.
+  Proof.
+    unfold indifferent_to_cast. intros Γ ϕ ψ e pf.
+    induction pf; unfold cast_proof; unfold eq_rec_r;
+      unfold eq_rec; unfold eq_rect; unfold eq_sym; simpl; auto;
+      pose proof (e' := e); move: e; rewrite e'; clear e'; intros e;
+      match type of e with
+      | ?x = ?x => replace e with (@erefl _ x) by (apply UIP_dec; intros x' y'; apply Pattern_eqdec)
+      end; simpl; try reflexivity.
   Qed.
 
   Definition indifferent_to_prop (P : proofbpred) :=
